src/lang/Configuration.v
@@ -151,7 +151,8 @@ Module Configuration.
       exploit Thread.rtc_step_disjoint; eauto. i. des.
       exploit Thread.step_disjoint; eauto. s. i. des.
       splits; ss. ii. apply CONSISTENT1; auto.
-      repeat (etrans; eauto).
+      + repeat (etrans; eauto).
+      + repeat (etrans; eauto).
     - s. apply WF0.
   Qed.
 
@@ -194,7 +195,8 @@ Module Configuration.
         exploit Thread.step_disjoint; eauto. s. i. des.
         splits; ss. inv CONSISTENT. exploit THREADS; eauto. i. des.
         ii. eapply CONSISTENT; eauto.
-        repeat (etrans; eauto).
+        * repeat (etrans; eauto).
+        * repeat (etrans; eauto).
       + apply WF0.
   Qed.
 
