src/opt/Composition.v
@@ -298,7 +298,10 @@ Proof.
   apply compose_consistent in CONSISTENT_SRC; auto.
   apply compose_consistent in CONSISTENT_TGT; auto.
   des. splits; i.
-  - punfold SIM1. exploit SIM1; eauto. i. des.
+  - punfold SIM1. exploit SIM1; eauto.
+    { i. eapply INTACT_SRC. rewrite Threads.compose_spec, H. ss. }
+    { i. eapply INTACT_TGT. rewrite Threads.compose_spec, H. ss. }
+    i. des.
     apply compose_is_terminal in TERMINAL_TGT; auto. des.
     exploit TERMINAL; eauto. i. des.
     exploit Configuration.rtc_step_consistent; eauto. s. i. des.
@@ -306,6 +309,8 @@ Proof.
     exploit compose_rtc_step1; eauto. s. i. des.
     punfold SIM2. exploit SIM2; eauto.
     { etrans; eauto. }
+    { admit. }
+    { admit. }
     i. des.
     exploit TERMINAL0; eauto. i. des.
     exploit Configuration.rtc_step_consistent; eauto. s. i. des.
@@ -317,7 +322,10 @@ Proof.
   - i. apply compose_step in STEP_TGT; auto. des; subst.
     + exploit Configuration.step_consistent; eauto. s. i. des.
       exploit Configuration.step_disjoint; eauto. s. i. des.
-      punfold SIM1. exploit SIM1; eauto. i. des.
+      punfold SIM1. exploit SIM1; eauto.
+      { i. eapply INTACT_SRC. rewrite Threads.compose_spec, H. ss. }
+      { i. eapply INTACT_TGT. rewrite Threads.compose_spec, H. ss. }
+      i. des.
       exploit STEP0; eauto. i. des; [|done].
       exploit Configuration.rtc_step_consistent; eauto. s. i. des.
       exploit Configuration.rtc_step_disjoint; eauto. s. i. des.
@@ -327,10 +335,17 @@ Proof.
       exploit compose_step1; eauto. i. des.
       eexists _, _, _, _. splits; eauto.
       right. apply CIH; auto.
-      eapply sim_future; eauto; repeat (etrans; eauto).
+      eapply sim_future; eauto.
+      * repeat (etrans; eauto).
+      * repeat (etrans; eauto).
+      * admit.
+      * admit.
     + exploit Configuration.step_consistent; eauto. s. i. des.
       exploit Configuration.step_disjoint; try symmetry; eauto. s. i. des.
-      punfold SIM2. exploit SIM2; eauto. i. des.
+      punfold SIM2. exploit SIM2; eauto.
+      { i. eapply INTACT_SRC. rewrite compose_comm, Threads.compose_spec, H; ss. }
+      { i. eapply INTACT_TGT. rewrite compose_comm, Threads.compose_spec, H; ss. }
+      i. des.
       exploit STEP0; eauto. i. des; [|done].
       exploit Configuration.rtc_step_consistent; eauto. s. i. des.
       exploit Configuration.rtc_step_disjoint; try symmetry; eauto. s. i. des.
@@ -341,5 +356,9 @@ Proof.
       eexists _, _, _, _. splits; eauto.
       right. apply CIH; auto.
       { symmetry. auto. }
-      eapply sim_future; eauto; repeat (etrans; eauto).
-Qed.
+      eapply sim_future; eauto.
+      * repeat (etrans; eauto).
+      * repeat (etrans; eauto).
+      * admit.
+      * admit.
+Admitted.
